\section{Manufactured solution}

\subsection{Finding f(x,y,t)}}

\begin{equation}
 u(x,y,t) = e^{-bt} \cos(\frac{m_x \pi}{L_x}) \cos(\frac{m_y \pi}{L_y}) \cos(\omega t)
 \label{standing_wave}
\end{equation}

Choose some $q(x,y) = A$ , $A \neq 0$ eq.(\ref{wave_eq}) becomes

\begin{equation}
 \frac{\partial^2 u}{\partial t^2} + v \frac{\partial u}{\partial t} = A \frac{\partial^2 u}{\partial x^2} + \frac{\partial^2 u}{\partial y^2} +f(x,y,t) 
\label{mod_wave_eq}
 \end{equation}



If we now insert eq.(\ref{standing_wave}) into eq.(\ref{mod_wave_eq}) we get

\begin{align*}
 \frac{\partial u}{\partial t} &= - b u(x,y,t) - \omega \underbrace{\frac{\sin(\omega t)}{\cos(\omega t)}}_{\tan(\omega t)}u(x,y,t) \\
 \frac{\partial^2 u}{\partial t^2} &= (b^2 -\omega^2) u(x,y,t) + 2\omega b \underbrace{\frac{\sin(\omega t)}{\cos(\omega t)}}_{\tan(\omega t)}u(x,y,t) \\
 \frac{\partial^2 u}{\partial x^2} &= - \left( \frac{m_x \pi}{L_x} \right)^2 u(x,y,t) \\
 \frac{\partial^2 u}{\partial y^2} &= - \left( \frac{m_y \pi}{L_y} \right)^2 u(x,y,t)
 \end{align*}
 
 \begin{align*}
  \Rightarrow \left[ (b^2 -\omega^2) + 2\omega b \tan(\omega t) - b^2 - b\omega \tan(\omega t) \right] u(x,y,t) = - A \left[ \left( \frac{m_x \pi}{L_x} \right)^2 + \left( \frac{m_y \pi}{L_y} \right)^2 \right] u(x,y,t) + f(x,y,t)\\
  \Rightarrow f(x,y,t) = \left[ \omega b \tan(\omega t) - \omega^2 + A \pi^2 \left( \left( \frac{m_x}{L_x} \right)^2 + \left( \frac{m_y}{L_y} \right)^2 \right) \right] u(x,y,t)
 \end{align*}

 \subsection{Finding I(x,y)}}

